13558/verify_program.v
@@ -1,0 +1,154 @@
+Require Import VST.floyd.proofauto.
+Require Import program.
+Instance CompSpecs : compspecs. make_compspecs prog. Defined.
+Definition Vprog : varspecs. mk_varspecs prog. Defined.
+
+Definition zip_with {A B C : Type} (f : A -> B -> C) (xs : list A) (ys : list B) : list C
+  := map (uncurry f) (combine xs ys).
+
+Definition sum_Z := fold_right Z.add 0.
+
+Lemma sum_Z_app xs ys : sum_Z (xs ++ ys) = sum_Z xs + sum_Z ys.
+Proof.
+  induction xs; simpl; lia.
+Qed.
+
+Lemma sum_Z_sublist (xs : list Z) (i : Z) :
+  0 <= i < Zlength xs -> sum_Z (sublist 0 (i+1) xs) = sum_Z (sublist 0 i xs) + Znth i xs.
+Proof.
+  intros.
+  rewrite (sublist_split 0 i (i+1)) by lia.
+  rewrite (sublist_one i (i+1)) by lia.
+  rewrite sum_Z_app; simpl.
+  lia.
+Qed.
+
+Lemma Zlength_combine (xs ys : list Z) :
+  Zlength (combine xs ys) = Z.min (Zlength xs) (Zlength ys).
+Proof.
+  apply Zlength_length.
+  list_solve.
+  rewrite combine_length.
+  rewrite Z2Nat.inj_min.
+  rewrite 2 ZtoNat_Zlength.
+  reflexivity.
+Qed.
+
+Lemma Znth_combine (xs ys : list Z) (i : Z) :
+  length xs = length ys ->
+  0 <= i < Zlength (combine xs ys) ->
+  Znth i (combine xs ys) = (Znth i xs, Znth i ys).
+Proof.
+  intros.
+  rewrite <- nth_Znth.
+  rewrite combine_nth.
+  rewrite 2 nth_Znth by (rewrite Zlength_combine in H0; lia).
+  reflexivity.
+  - lia.
+  - lia.
+Qed.
+
+Definition flipped_inner_product (xs ys : list Z) : Z :=
+  sum_Z (zip_with Z.mul xs (rev ys)).
+
+Definition flipped_inner_product_spec : ident * funspec :=
+  DECLARE _flipped_inner_product
+    WITH xs_sh : share, ys_sh : share, xs_ptr : val, ys_ptr : val, xs : list Z, ys : list Z, size : Z
+    PRE [ tptr tuint, tptr tuint, tulong ]
+      PROP (
+        readable_share xs_sh;
+        readable_share ys_sh;
+        0 <= size <= Int64.max_unsigned;
+        Forall (fun x => 0 <= x <= Int.max_unsigned) xs;
+        Forall (fun x => 0 <= x <= Int.max_unsigned) ys
+      )
+      PARAMS (xs_ptr; ys_ptr; Vlong (Int64.repr size))
+      SEP (
+        data_at xs_sh (tarray tuint size) (map (Vint oo Int.repr) xs) xs_ptr;
+        data_at ys_sh (tarray tuint size) (map (Vint oo Int.repr) ys) ys_ptr
+      )
+    POST [ tulong ]
+      PROP ()
+      RETURN (Vlong (Int64.repr (flipped_inner_product xs ys)))
+      SEP (
+        data_at xs_sh (tarray tuint size) (map (Vint oo Int.repr) xs) xs_ptr;
+        data_at ys_sh (tarray tuint size) (map (Vint oo Int.repr) ys) ys_ptr
+      ).
+
+Definition Gprog := [ flipped_inner_product_spec ].
+
+Lemma body_flipped_inner_product_spec :
+  semax_body Vprog Gprog f_flipped_inner_product flipped_inner_product_spec.
+Proof.
+  start_function.
+  forward.
+  forward_for_simple_bound size (
+    EX i : Z,
+      PROP (
+        readable_share xs_sh;
+        readable_share ys_sh;
+        i <= size
+      )
+      LOCAL (
+        temp _sum (Vlong (Int64.repr (sum_Z (sublist 0 i (map (uncurry Z.mul) (combine xs (rev ys)))))));
+        temp _xs xs_ptr;
+        temp _ys ys_ptr;
+        temp _n (Vlong (Int64.repr size))
+      )
+      SEP (
+            data_at xs_sh (tarray tuint size) (map (Vint oo Int.repr) xs) xs_ptr;
+            data_at ys_sh (tarray tuint size) (map (Vint oo Int.repr) ys) ys_ptr
+      )).
+  - entailer!.
+  - assert_PROP (0 <= i < Zlength xs) by (entailer!; list_solve).
+    forward.
+    assert_PROP (0 <= size - i - 1 < Zlength ys) by (entailer!; list_solve).
+    forward.
+    forward.
+    entailer!.
+    remember (map (uncurry Z.mul) (combine xs (rev ys))) as lst.
+    rewrite sum_Z_sublist.
+    repeat (rewrite Zlength_map in *).
+    rewrite <- H9.
+    rewrite <- Znth_rev in *.
+    + rewrite Heqlst.
+      rewrite Znth_map.
+      rewrite Znth_combine.
+      simpl.
+      rewrite 2 Int.unsigned_repr.
+      reflexivity.
+      * apply sublist.Forall_Znth.
+        rewrite Zlength_rev.
+        lia.
+        apply Forall_rev.
+        assumption.
+      * apply sublist.Forall_Znth.
+        lia.
+        assumption.
+      * rewrite rev_length.
+        rewrite 2 Zlength_correct in H9.
+        lia.
+      * rewrite Zlength_combine.
+        rewrite Zlength_rev.
+        lia.
+      * rewrite Zlength_combine.
+        rewrite Zlength_rev.
+        lia.
+    + lia.
+    + rewrite Heqlst.
+      repeat (rewrite Zlength_map in *).
+      rewrite Zlength_combine.
+      rewrite Zlength_rev.
+      lia.
+  - forward.
+    entailer!.
+    unfold flipped_inner_product, zip_with.
+    rewrite Zlength_map in *.
+    rewrite sublist_same.
+    + reflexivity.
+    + reflexivity.
+    + repeat (rewrite Zlength_map in *).
+      rewrite Zlength_combine.
+      rewrite Zlength_rev.
+      lia.
+Qed.
